sep7notes.lean
@@ -1,0 +1,73 @@
+#check Empty -- no values computational
+#check False -- no proofs logical
+
+#check Unit --one value, like void in java? computational
+#check True -- logical, one value = proof
+
+example : Nat := 2
+example : True := True.intro
+example: Unit := Unit.unit
+
+namespace hidden
+
+inductive Bool : Type where
+| true : Bool
+| false : Bool
+
+
+def b2s (b : Bool) : String :=
+  match b with -- must enumarate all cases
+  | Bool.true => "true"
+  | Bool.false => "false"
+
+end hidden
+
+
+#check Bool -- two values
+
+#check Option Bool --
+
+#check Nat -- natural numbers
+
+
+namespace hidden
+
+inductive Nat : Type where
+| Zero : Nat
+| Succ (n: Nat) : Nat
+
+
+
+
+open hidden.Nat
+
+def zero : Nat := Nat.Zero
+def one : Nat := Nat.Succ zero
+def two : Nat := Nat.Succ one
+
+def funk (n : Nat) : String :=
+  match n with
+  | Nat.Zero => ""
+  | Nat.Succ n' => "!" ++ funk n'
+
+
+#eval funk two
+
+end hidden
+
+#check Prod
+#check Sum
+
+
+def id_Empty : Empty → Empty :=
+  fun x => x
+def id_ListNat : List Nat → List Nat :=
+  fun x => x
+
+def swap'' :
+∀
+  (α : Type u)
+  (β : Type u),
+  a × b → b × a
+  :=
+  fun α β (a, b) => (b, a)
